

$$C_l = \frac{l}{\frac{1}{2}\rho_{\infty}U_{\infty}^2c} = \frac{l}{\frac{1}{2}\gamma P_{\infty}M_{\infty}^2c}$$

$$C_d = \frac{d}{\frac{1}{2}\rho_{\infty}U_{\infty}^2c} = \frac{d}{\frac{1}{2}\gamma P_{\infty}M_{\infty}^2c}$$

$$l = P_3 z \cos(\theta + \alpha) + P_4 z \cos(\theta - \alpha) - P_1 z \cos(\theta - \alpha) - P_2 z \cos(\theta + \alpha)$$

$$d = P_1 z \sin(\theta + \alpha) + P_3 z \sin(\theta - \alpha) - P_2 z \sin(\theta - \alpha) - P_4 z \sin(\theta + \alpha)$$

$$C_l = \frac{z}{\frac{1}{2}\gamma P_{\infty}M_{\infty}^2c} [(P_3 - P_2)\cos(\theta + \alpha) + (P_4 - P_1)\cos(\theta - \alpha)]$$

$$C_d = \frac{z}{\frac{1}{2}\gamma P_{\infty}M_{\infty}^2c} [(P_1 - P_4)\sin(\theta - \alpha) + (P_3 - P_2)\sin(\theta + \alpha)]$$

$$z = \frac{(c/2)}{\cos(\theta)}$$

$$C_l = \frac{1}{\gamma P_{\infty}M_{\infty}^2 \cos(\theta)} [(P_3 - P_2)\cos(\theta + \alpha) + (P_4 - P_1)\cos(\theta - \alpha)]$$

$$C_d = \frac{1}{\gamma P_{\infty}M_{\infty}^2 \cos(\theta)} [(P_1 - P_4)\sin(\theta - \alpha) + (P_3 - P_2)\sin(\theta + \alpha)]$$

